expand on proof of concept, prove sum program is optimal

ProofOfConcept.v
@@ -5,36 +5,80 @@ Import ListNotations.
 Local Open Scope Z_scope.
 
 (* Implementation of maps is left abstract for now *)
-Class map_impl :=
+Class map_impl A :=
   {
-    map : forall A B : Type, Type;
-    get : forall {A B}, map A B -> A -> B;
-    update : forall {A B}, map A B -> A -> B -> map A B;
-    empty : forall A B (default:B), map A B;
-    get_empty : forall A B d a, get (empty A B d) a = d;
-    get_update_eq : forall A B a b (m : map A B), get (update m a b) a = b;
-    get_update_neq : forall A B a1 a2 b (m : map A B), a1 <> a2 -> get (update m a1 b) a2 = get m a2;
+    map : forall B : Type, Type;
+    get : forall {B}, map B -> A -> B;
+    update : forall {B}, map B -> A -> B -> map B;
+    empty : forall {B} (default:B), map B;
+    get_empty : forall B (d:B) a, get (empty d) a = d;
+    get_update_eq : forall B a b (m : map B), get (update m a b) a = b;
+    get_update_neq : forall B a1 a2 b (m : map B), a1 <> a2 -> get (update m a1 b) a2 = get m a2;
   }.
+Arguments map _ {_} _.
+
+(* Util : eventually will be in a separate file *)
+Module Z.
+  Lemma pow_base_lt a b : 1 < a -> 1 < b -> a < a ^ b.
+  Proof.
+    intros. apply Z.le_lt_trans with (m:=a^1); [ rewrite Z.pow_1_r; lia | ].
+    apply Z.pow_lt_mono_r; lia.
+  Qed.
+End Z.
+Lemma map_nil {A B} (f:A -> B): List.map f [] = []. Proof. reflexivity. Qed.
+Lemma nth_default_nil {A} (d:A) i : nth_default d [] i = d. Proof. destruct i; reflexivity. Qed.
+Lemma nth_default_cons_0 {A} (d:A) l0 l : nth_default d (l0 :: l) 0 = l0. Proof. reflexivity. Qed.
+Lemma nth_default_cons_S {A} (d:A) l0 l i : nth_default d (l0 :: l) (S i) = nth_default d l i. Proof. reflexivity. Qed.
+Lemma length_nil {A} : length (@nil A) = 0%nat. Proof. reflexivity. Qed.
+Lemma length_cons {A} (a0 : A) l : length (a0 :: l) = S (length l). Proof. reflexivity. Qed.
+Hint Rewrite @get_update_eq @get_empty @get_update_neq using congruence :  push_mapt.
+Hint Rewrite @map_cons @map_nil : push_map.
+Hint Rewrite @nth_default_nil @nth_default_cons_0 @nth_default_cons_S : push_nth_default.
+Hint Rewrite @length_nil @length_cons : distr_length.
+Ltac solve_zrange :=
+  solve [repeat match goal with
+                | |- _ /\ _ => split
+                | _ => lia
+                | _ => apply Z.div_le_lower_bound
+                | _ => apply Z.div_lt_upper_bound
+                | _ => apply Z.div_le_upper_bound
+                end].
+Ltac zero_bounds :=
+  repeat match goal with
+           | _ => lia
+           | |- _ >= 0 => apply Z.ge_le
+           | |- _ > 0 => apply Z.gt_lt
+           | |- 0 < _ ^ _ => apply Z.pow_pos_nonneg
+           | |- 0 <= Z.of_nat _ => apply Nat2Z.is_nonneg
+           | |- 1 < _ ^ _ => apply Z.pow_gt_1
+         end.
+Ltac distr_length :=
+  autorewrite with distr_length in *; try lia.
+(* TODO: improve *)
+Ltac break_match :=
+  match goal with
+  | |- context [match ?x with _ => _ end] => destruct x
+  end.
+
 
 (* Machine model *)
 Module Machine.
   Section Machine.
-    Context {mapt : map_impl}. (* we use abstract maps to keep track of state *)
     Context {register flag instruction : Set}.
+    Context {reg_mapt : map_impl register} {flag_mapt : map_impl flag}. (* we use abstract maps to keep track of state *)
     Context {register_size : register -> nat}
-            {register_value : (map register Z) -> register -> Z}
             {flag_spec : nat (* destination register size *) -> flag -> Z -> bool}.
-    Context {cost : instruction -> nat}
-            {flags_written : instruction -> list flag}
+    Context {flags_written : instruction -> list flag}
             {spec : instruction -> list Z -> (flag -> bool) -> Z}
-            {precondition : instruction -> register -> list register -> Prop}.
+            {precondition : instruction -> register -> list (register + Z) -> Prop}.
+    Local Notation arg := (register + Z)%type.
 
     Inductive program : Type :=
     | Ret : register -> program
     | Instr :
         instruction ->
         register (* destination *) ->
-        list register (* arguments *) ->
+        list arg (* arguments *) ->
         program (* continuation *) ->
         program
     .
@@ -47,11 +91,17 @@ Module Machine.
         valid (Instr i rd args cont)
     .
 
+    Definition arg_value (ctx : map register Z) (x:arg) : Z :=
+      match x with
+      | inl r => get ctx r
+      | inr z => z
+      end.
+
     Fixpoint exec (e : program) (ctx : map register Z) (flag_ctx : map flag bool) : Z :=
       match e with
       | Ret r => get ctx r
       | Instr i rd args cont =>
-        let result := i.(spec) (List.map (register_value ctx) args) (get flag_ctx) in
+        let result := i.(spec) (List.map (arg_value ctx) args) (get flag_ctx) in
         let n := register_size rd in
         let ctx' := update ctx rd (result mod 2^(Z.of_nat n)) in
         let flag_ctx' :=
@@ -59,20 +109,14 @@ Module Machine.
         exec cont ctx' flag_ctx'
       end.
 
-    Fixpoint get_cost (e : program) : nat :=
-      match e with
-      | Ret r => 0
-      | Instr i rd args cont => i.(cost) + get_cost cont
-      end.
-
     Definition valid_context (ctx : map register Z) := forall r, 0 <= get ctx r < 2^ (Z.of_nat (register_size r)).
 
   End Machine.
 
   Module Notations.
-    Notation "i rd x ; p" := (Instr i rd (x :: nil) p) (at level 100, p at level 200, format "i  rd  x ; '//' p").
-    Notation "i rd x y ; p" := (Instr i rd (x :: y :: nil) p) (at level 100, p at level 200, format "i  rd  x  y ; '//' p").
-    Notation "i rd x y z ; p" := (Instr i rd (x :: y :: z :: nil) p) (at level 100, p at level 200, format "i  rd  x  y  z ; '//' p").
+    Notation "i % rd x ; p" := (Instr i rd (x :: nil) p) (at level 100, p at level 200, format "i  % rd  x ; '//' p").
+    Notation "i % rd x y ; p" := (Instr i rd (x :: y :: nil) p) (at level 100, p at level 200, format "i  % rd  x  y ; '//' p").
+    Notation "i % rd x y z ; p" := (Instr i rd (x :: y :: z :: nil) p) (at level 100, p at level 200, format "i  % rd  x  y  z ; '//' p").
   End Notations.
 End Machine.
 
@@ -87,7 +131,7 @@ End Flags.
 
 Module Instructions.
   Section Instructions.
-    Context {register : Set} {size : register -> nat}.
+    Context {register : Set} {register_size : register -> nat}.
 
     Local Notation "x '[' n ']'" := (List.nth_default 0 x n) (at level 0).
     Local Notation "x >> y" := (Z.shiftr x y) (at level 100).
@@ -126,12 +170,40 @@ Module Instructions.
       | MOV64 => 1
       end.
 
-    Definition precondition (i:instruction) (rd:register) (args:list register) : Prop :=
+    Definition arg_size (x : register + Z) : nat :=
+      match x with
+      | inl r => register_size r
+      | inr z =>
+        if Z_lt_dec z 0
+        then 0
+        else Pos.to_nat (Pos.size (Z.to_pos z))
+      end.
+
+    Definition precondition (i:instruction) (rd:register) (args:list (register + Z)) : Prop :=
       length args = num_source_regs i
-      /\ Forall (fun r => (size r <= instr_size i)%nat) args
-      /\ (size rd >= instr_size i)%nat.
- 
-    Definition cost (i:instruction) : nat :=
+      /\ Forall (fun r => (0 < arg_size r <= instr_size i)%nat) args
+      /\ (register_size rd >= instr_size i)%nat.
+  End Instructions.
+End Instructions.
+
+Module Registers.
+  Inductive register : Set := r0 | r1 | r2 | r3 | r4 | r5 | r6.
+  Definition size (r:register) : nat :=
+    match r with
+    | r0 | r1 => 32%nat
+    | r2 | r3 | r4 | r5 | r6 => 64%nat
+    end.
+  Notation "$ y" := (@inr register Z y) (at level 40, format "$ y").
+  Notation "% r" := (@inl register Z r) (at level 40, format "% r").
+End Registers.
+
+Module CostModel.
+  Import Instructions.
+  Section CostModel.
+    Context {register : Set} {size : register -> nat}.
+    Local Notation program := (Machine.program (register:=register) (instruction:=instruction)).
+
+    Definition instr_cost (i:instruction) : nat :=
       match i with
       | ADD32 => 2
       | ADD64 | ADC64 | SUB64 => 4
@@ -139,95 +211,125 @@ Module Instructions.
       | SHR64 | SHL64 => 2
       | MOV64 => 1
       end.
-    
-  End Instructions.
-End Instructions.
+    Fixpoint cost (p : program) : nat :=
+      match p with
+      | Machine.Ret r => 0
+      | Machine.Instr i rd args cont => i.(instr_cost) + cost cont
+      end.
 
-Module Registers.
-  Inductive register : Set := r0 | r1 | r2 | r3 | r4 | r5 | r6 | const : Z -> register.
-  Definition size (r:register) : nat :=
-    match r with
-    | r0 | r1 => 32%nat
-    | r2 | r3 | r4 | r5 | r6 => 64%nat
-    | const x => Z.to_nat (Z.log2 x)
-    end.
-  Definition value {mapt : map_impl} (ctx : map register Z) (r:register) : Z :=
-    match r with
-    | const x => x
-    | _ => get ctx r
-    end.
-  Notation "'#' y" := (const y) (at level 30, format "# y").
-End Registers.
+    Definition optimal (equiv : program -> program -> Prop) (p : program) : Prop :=
+      forall p' : program,
+        Machine.valid (precondition:=precondition (register_size:=size)) p'
+        -> (equiv p p')
+        -> (cost p <= cost p')%nat.
+  End CostModel.
+End CostModel.
+
+
+Module Maps.
+  Module Generic.
+    Section Generic.
+      Context {A : Type} {A_eq_dec : forall a1 a2 : A, {a1 = a2} + {a1 <> a2} }.
+
+      Inductive t {B} : Type :=
+      | Empty : B -> t
+      | Update : t -> A -> B -> t
+      .
+
+      Fixpoint get {B} (m : @t B) (k : A) : B :=
+        match m with
+        | Empty d => d
+        | Update m' a b => if A_eq_dec k a then b else get m' k
+        end.
+
+      Instance impl : map_impl A.
+      Proof.
+        apply Build_map_impl with (map:=@t) (get:=@get) (update:=@Update) (empty:=@Empty).
+        { reflexivity. }
+        { intros; cbn. break_match; congruence. }
+        { intros; cbn. break_match; congruence. }
+      Defined.
+    End Generic.
+  End Generic.
+
+  Lemma get_update_full
+        {A B} {mapt : map_impl A}
+        {A_eq_dec : forall a1 a2 : A, {a1 = a2} + {a1 <> a2}}
+        (m: map A B) a1 a2 b:
+    get (update m a1 b) a2 = if A_eq_dec a1 a2 then b else get m a2.
+  Proof. break_match; subst; autorewrite with push_mapt; reflexivity. Qed.
+
+  Definition reg_eq_dec (r1 r2 : Registers.register) : {r1 = r2} + {r1 <> r2}.
+  Proof.
+    destruct r1, r2; try (left; congruence); right; congruence.
+  Defined.
+
+  Definition flag_eq_dec (f1 f2 : Flags.flag) : {f1 = f2} + {f1 <> f2}.
+  Proof.
+    destruct f1, f2; try (left; congruence); right; congruence.
+  Defined.
+
+  Instance reg_mapt : map_impl Registers.register := @Generic.impl _ reg_eq_dec.
+  Instance flag_mapt : map_impl Flags.flag := @Generic.impl _ flag_eq_dec.
+End Maps.
 
 Module Glue.
-  Section with_mapt.
-    Context {mapt : map_impl}.
-    Definition exec := Machine.exec
-                         (register_size:=Registers.size)
-                         (register_value:=Registers.value)
-                         (flag_spec:=Flags.flag_spec)
-                         (flags_written:=Instructions.flags_written)
-                         (spec:=Instructions.spec).
-    Definition valid := Machine.valid
+  Import Maps.
+  Definition exec := Machine.exec
+                       (register_size:=Registers.size)
+                       (flag_spec:=Flags.flag_spec)
+                       (flags_written:=Instructions.flags_written)
+                       (spec:=Instructions.spec).
+  Definition valid := Machine.valid
+                        (register:=Registers.register)
+                        (precondition:=Instructions.precondition
+                                         (register_size:=Registers.size)).
+  Definition program := Machine.program
                           (register:=Registers.register)
-                          (precondition:=Instructions.precondition (size:=Registers.size)).
-    Definition program := Machine.program (register:=Registers.register) (instruction:=Instructions.instruction).
-    Definition valid_context := Machine.valid_context
-                                  (register:=Registers.register)
-                                  (register_size:=Registers.size).
-  End with_mapt.
-
-  (* equivalence is quantified over all implementations of map *)
+                          (instruction:=Instructions.instruction).
+  Definition valid_context := Machine.valid_context
+                                (register:=Registers.register)
+                                (register_size:=Registers.size).
+  Definition precondition := Instructions.precondition (register_size:=Registers.size).
   Definition equivalent (p1 p2 : program) :=
-    forall (mapt : map_impl) ctx fctx,
+    forall ctx fctx,
       valid_context ctx ->
       exec p1 ctx fctx = exec p2 ctx fctx.
   Infix "==" := equivalent (at level 100).
+  Definition optimal := CostModel.optimal (size:=Registers.size) equivalent.
 End Glue.
 
 Module Examples.
-  Import Instructions. Import Machine. Import Registers.
-  Import Machine.Notations. Import Glue.
+  Import Instructions. Import Machine. Import Registers. Import CostModel.
+  Import Machine.Notations. Import Maps. Import Glue.
 
   Definition examples : list program :=
     [
       (Ret r0); (* simplest program *)
 
         (* move value in r3 to r2 and return it *)
-        (Instr MOV64 r2 (r3 :: nil) (Ret r2));
+        (Instr MOV64 r2 (%r3 :: nil) (Ret r2));
         
         (* r0 + r1 with 32-bit add, result in r0 *)
-        (Instr ADD32 r0 (r0 :: r1 :: nil) (Ret r0));
+        (Instr ADD32 r0 (%r0 :: %r1 :: nil) (Ret r0));
 
         (* r0 + r1 with 32-bit add, result in r2 (which is oversized) *)
-        (Instr ADD32 r2 (r0 :: r1 :: nil) (Ret r2));
+        (Instr ADD32 r2 (%r0 :: %r1 :: nil) (Ret r2));
 
         (* r0 + r1 with 64-bit add, result in r2 *)
-        (Instr ADD64 r2 (r0 :: r1 :: nil) (Ret r2));
+        (Instr ADD64 r2 (%r0 :: %r1 :: nil) (Ret r2));
 
         (* (r0 + r1) >> 1 with 32-bit add, result in r2 *)
-        (Instr ADD32 r2 (r0 :: r1 :: nil) (Instr SHR64 r2 (r2 :: #1 :: nil) (Ret r2)));
+        (Instr ADD32 r2 (%r0 :: %r1 :: nil) (Instr SHR64 r2 (%r2 :: $1 :: nil) (Ret r2)));
 
         (* (r0 + r1) >> 1 with 64-bit add, result in r2 *)
-        (Instr ADD64 r2 (r0 :: r1 :: nil) (Instr SHR64 r2 (r2 :: #1 :: nil) (Ret r2)))
+        (Instr ADD64 r2 (%r0 :: %r1 :: nil) (Instr SHR64 r2 (%r2 :: $1 :: nil) (Ret r2)))
     ].
 
   Lemma examples_valid : Forall valid examples.
   Proof. repeat econstructor. Qed.
 
-  Lemma map_nil {A B} (f:A -> B): List.map f [] = []. Proof. reflexivity. Qed.
-  Lemma nth_default_nil {A} (d:A) i : nth_default d [] i = d. Proof. destruct i; reflexivity. Qed.
-  Lemma nth_default_cons_0 {A} (d:A) l0 l : nth_default d (l0 :: l) 0 = l0. Proof. reflexivity. Qed.
-  Lemma nth_default_cons_S {A} (d:A) l0 l i : nth_default d (l0 :: l) (S i) = nth_default d l i. Proof. reflexivity. Qed.
-  Hint Rewrite @get_update_eq @get_empty : push_mapt.
-  Hint Rewrite @map_cons @map_nil : push_map.
-  Hint Rewrite @nth_default_nil @nth_default_cons_0 @nth_default_cons_S : push_nth_default.
-
-  (* prove sum using 32- and 64- bit adds give the same result *)
-  Definition sum := Eval compute in (nth_default (Ret r0) examples 5). (* ADD32 r2 r0 r1; SHR64 r2 r2 #1; Ret r2 *)
-  Definition sum' := Eval compute in (nth_default (Ret r0) examples 6). (* ADD64 r2 r0 r1; SHR64 r2 r2 #1; Ret r2 *)
-
-  Lemma valid_context_range {mapt: map_impl} ctx r :
+  Lemma valid_context_range ctx r :
     valid_context ctx -> 0 <= get ctx r < 2 ^ (Z.of_nat (Registers.size r)).
   Proof. auto. Qed.
 
@@ -241,32 +343,172 @@ Module Examples.
                 end)
     end.
 
-  Ltac solve_zrange :=
-    solve [repeat match goal with
-                  | |- _ /\ _ => split
-                  | _ => lia
-                  | _ => apply Z.div_le_lower_bound
-                  | _ => apply Z.div_lt_upper_bound
-                  | _ => apply Z.div_le_upper_bound
-                  end].
-  
+  Hint Unfold
+       equivalent exec Machine.exec 
+       optimal CostModel.optimal CostModel.cost CostModel.instr_cost
+       precondition Instructions.precondition.
+  Ltac simplify := autounfold; cbn [size value spec arg_value].
 
-  Hint Unfold equivalent exec Machine.exec size spec value.
-  Hint Unfold sum sum'.
-  
-  Lemma sums_equiv : sum == sum'.
-  Proof.
-    repeat match goal with
-           | _ => progress (intros; autounfold)
-           | _ => progress autorewrite with push_map push_mapt push_nth_default
-           | _ => progress pose_valid_context_range
-           | |- context [?a mod ?b] => rewrite (Z.mod_small a b) by lia
-           end.
-    rewrite Z.shiftr_div_pow2, Z.pow_1_r by lia.
-    rewrite !Z.mod_small by solve_zrange.
-    reflexivity.
-  Qed.
-End Examples.
+  (* prove sum using 32- and 64- bit adds give the same result *)
+  Section SumEquiv.
+    Definition sum :=
+      Eval compute in (nth_default (Ret r0) examples 5). (* ADD32 r2 r0 r1; SHR64 r2 r2 #1; Ret r2 *)
+    Definition sum' :=
+      Eval compute in (nth_default (Ret r0) examples 6). (* ADD64 r2 r0 r1; SHR64 r2 r2 #1; Ret r2 *)
+    Hint Unfold sum sum'.
     
+    Lemma sums_equiv : sum == sum'.
+    Proof.
+      repeat match goal with
+             | _ => progress (intros; autounfold; simplify)
+             | _ => progress autorewrite with push_map push_mapt push_nth_default
+             | _ => progress pose_valid_context_range
+             | |- context [?a mod ?b] => rewrite (Z.mod_small a b) by lia
+             end.
+      reflexivity.
+    Qed.
+  End SumEquiv.
+
+  (* Prove that programs are optimal *)
+  Section Optimal.
+    Definition simple_sum :=
+      Eval compute in (nth_default (Ret r0) examples 3). (* ADD32 r2 r0 r1; Ret r2 *)
+    Hint Unfold simple_sum.
+
+    (* TODO: move all this somewhere (costmodelproofs?) *)
+    Definition min_instr_cost : nat := 1.
+    Lemma min_instr_cost_correct : forall i, (min_instr_cost <= instr_cost i)%nat.
+    Proof. intros; destruct i; cbv [min_instr_cost instr_cost]; lia. Qed.
+    Fixpoint depth (p : program) : nat :=
+      match p with
+      | Ret _ => 0
+      | Instr _ _ _ cont => S (depth cont)
+      end.
+    Lemma depth_min_cost :
+      forall p, ((depth p) * min_instr_cost <= cost p)%nat.
+    Proof.
+      induction p; intros; [ reflexivity | ]. cbn [depth cost].
+      pose proof min_instr_cost_correct i. lia.
+    Qed.
+    Lemma length_args i rd args cont : valid (Instr i rd args cont) -> length args = i.(num_source_regs).
+    Proof. inversion 1; intros; subst. autounfold in *. tauto. Qed.
+
+    (* TODO: move to InstructionProofs *)
+    (* TODO: simplify/automate; probably want a push_pos2z tactic, etc *)
+    Lemma arg_size_constant_upper_bound x u :
+      (0 < arg_size (register_size:=Registers.size) ($x) <= u)%nat ->
+      0 <= x < 2 ^ Z.of_nat u.
+    Proof.
+      cbv [arg_size]; break_match; intro Hrange;
+        destruct Hrange as [Hlower Hupper]; [lia | split; [ lia | ] ].
+      destruct (Z.eq_dec x 0); (* Z->positive proofs want x > 0 *)
+        [ subst; apply Z.pow_pos_nonneg; lia | ].
+      eapply Z.le_lt_trans with (m:=Z.pos (Z.to_pos x));
+        [rewrite Z2Pos.id by lia; reflexivity | ].
+      eapply Z.lt_le_trans with (m:=Z.pos (2^(Pos.size (Z.to_pos x)))).
+      { auto using Pos2Z.pos_lt_pos, Pos.size_gt. }
+      { rewrite Pos2Z.inj_pow.
+        apply Z.pow_le_mono_r; [ lia | ].
+        apply inj_le in Hupper.
+        rewrite positive_nat_Z in Hupper.
+        lia. }
+    Qed.
+
+    Local Ltac prove_valid_ctx :=
+      econstructor; autorewrite with push_mapt;
+      rewrite ?(get_update_full (A_eq_dec:=reg_eq_dec)); cbv [size];
+      repeat break_match; subst; autorewrite with push_mapt; lia.
+    Local Ltac destruct_args :=
+      match goal with H : Machine.valid (Instr _ _ ?args _) |- _ =>
+                      let H' := fresh in
+                      pose proof (length_args _ _ _ _ H) as H';
+                      cbv [num_source_regs] in H';
+                      repeat (destruct args as [|? args]; distr_length)
+      end; repeat match goal with H : ?x = ?x |- _ => clear H end.
+    Local Ltac inversion_Forall :=
+      repeat match goal with
+             | H : Forall _ (?x :: _) |- _ =>
+               let a := fresh "a" in
+               let l := fresh "l" in
+               inversion H as [ | a l ] ; clear H; subst a; subst l
+             | H : Forall _ [] |- _ => clear H
+             end.
+    Local Ltac inversion_valid :=
+      repeat
+        (match goal with
+             | H : Machine.valid (Instr ?i ?rd ?args ?cont) |- _ =>
+               inversion H; clear H;
+               try match goal with H' : ?x = i |- _ => subst x end;
+               try match goal with H' : ?x = rd |- _ => subst x end;
+               try match goal with H' : ?x = args |- _ => subst x end;
+               try match goal with H' : ?x = cont |- _ => subst x end
+         end;
+         repeat match goal with
+                | H : Instructions.precondition _ _ _ |- _ =>
+                  let H' := fresh in
+                  inversion H as [? H']; clear H;
+                  repeat match type of H' with
+                           _ /\ _ =>
+                           let H'':= fresh in destruct H' as [H'' H']
+                         end
+                | _ => progress inversion_Forall
+                | _ => progress autorewrite with distr_length in *
+                | _ => progress cbn [instr_size num_source_regs] in *
+                end).
+    Local Ltac pose_not_equivalent :=
+      match goal with H : ?p1 == ?p2 |- _ =>
+                      let H' := fresh in
+                      assert (exists ctx, exec p1 ctx (empty false) <>
+                                          exec p2 ctx (empty false)
+                                          /\ valid_context ctx) as H';
+                      [| destruct H' as [? [H' ?] ]; solve [auto] ]
+      end.
+    Lemma simple_sum_optimal : optimal simple_sum.
+    Proof.
+      repeat intro.
+      assert (forall r, 2 < 2 ^ Z.of_nat (size r)).
+      { destruct r; cbn [size]; apply Z.pow_base_lt; lia. }
+      repeat match goal with
+             | p : Machine.program |- _ =>
+               destruct p as [? | i]; [ | destruct i ];
+                 try solve [simplify; lia]
+             end;
+        exfalso; try destruct_args; pose_not_equivalent.
+      (* leaves us with all programs that are strictly lower-cost than
+      simple_sum -- Ret and MOV/Ret *)
+      (* based on the unknown registers/arguments in context,
+            construct counterexample contexts. Eventually, this should
+            be done more automatically. *)
+      1: (exists (update (update (empty 0) r0 1) r1 1)).
+      2: match goal with
+         | a : register + Z |- _ =>
+           exists (update (update (empty 0) r0 1) r1
+                          (match a with
+                           | inr z => if Z.eq_dec z 2 then 2 else 1
+                           | _ => 1
+                           end))
+         end.
+      all: split; [ | solve [prove_valid_ctx] ]; autounfold; simplify;
+        autorewrite with push_map push_nth_default push_mapt.
+      all:repeat match goal with
+                 | _ => break_match; subst
+                 | _ => progress simplify
+                 | _ => progress autorewrite with push_mapt
+                 | H : _ |- _ => apply arg_size_constant_upper_bound in H
+                 | _ => rewrite (get_update_full (A_eq_dec := reg_eq_dec))
+                 | H : context[forall r, _ < 2 ^ (Z.of_nat (size r))]
+                   |- context [?x mod 2 ^ (Z.of_nat (size ?r))] =>
+                   rewrite (Z.mod_small x (2 ^ (Z.of_nat (size r)))) by
+                       (specialize (H r); lia)
+                 | H : context [?x < ?a ^ ?b] |- context [?x mod ?a ^ ?c] =>
+                   rewrite (Z.mod_small x (a ^ c))
+                     by (pose proof (Z.pow_le_mono_r 2 b c); lia)
+                 | _ => rewrite Z.mod_small by lia
+                 | _ => lia
+                 | _ => progress inversion_valid
+                 end.
+    Qed.
+  End Optimal.
+End Examples.
     
     
